incomplete proof

X3dh/Basic.lean
@@ -17,8 +17,8 @@ instance : ToString Kind where
    | .prv => "private"
 
 def Kind.rev : Kind → Kind
-| .pub => .prv
-| .prv => .pub
+ | .pub => .prv
+ | .prv => .pub
 
 -- a structure to hold a Key
 structure Key where
@@ -30,10 +30,11 @@ structure Key where
 instance : ToString Key where
   toString k := s!"{k.userName}_{k.label}_{k.kind}"
 
+
 def match_key (k1 k2 : Key) : Bool :=
-  k1.kind.rev = k2.kind
-  ∧ k1.userName = k2.userName
+  k1.userName = k2.userName
   ∧ k1.label = k2.label
+  ∧ k1.kind.rev = k2.kind
 
 
 inductive ByteSequence where
@@ -68,6 +69,7 @@ def match_bs (b1 b2 : ByteSequence) : Bool :=
 structure KeyPair where
   privateKey : Key
   publicKey  : Key
+  valid      : match_key privateKey publicKey
  deriving Repr
 
 
@@ -81,7 +83,8 @@ structure Agent where
 
 def generateKeyPair (name : AgentName) (label : String) : KeyPair :=
   { privateKey := Key.mk name label Kind.prv,
-    publicKey := Key.mk name label Kind.pub }
+    publicKey  := Key.mk name label Kind.pub,
+    valid      := by simp [match_key]; rfl }
 
 structure Registry where
   agents : List Agent
@@ -242,16 +245,75 @@ def receiveInitMessage  (receiver : Agent) (msg : Message)
   | Except.error s => Except.error s
 
 
-theorem commonSharedSecret {a b : Agent} {txt : String} (msg : Message) :
-   sendInitMessage a b txt = Except.ok msg →
-   receiveInitMessage b msg = Except.ok txt := by
-   intro h
-   simp [sendInitMessage, receiveInitMessage,
-     toPublicBundle, toPrivateBundle, deriveSharedSecret,
-     decrypt, encrypt,
-     ByteSequence.append, makeMessage, verify,
-     match_bs, match_key] at *
-   sorry
+-- for all agents A and all KeyPairs K ~> match_key k k.rev
+
+theorem all_agentIK₁ :
+  ∀ (a : Agent) (k : KeyPair), a.IK = k → match_key k.privateKey k.publicKey := by
+  intro a k h₁
+  have h₂ := k.valid
+  exact h₂
+
+theorem all_agentIK₂ :
+  ∀ (a : Agent), match_key a.IK.privateKey a.IK.publicKey := by
+  intro a
+  let h₁ := a.IK
+  let k1 := a.IK.publicKey
+  let k2 := a.IK.privateKey
+  let h₂ := h₁.valid
+  exact h₂
+
+theorem all_agentSPK₂ :
+  ∀ (a : Agent), match_key a.SPK.privateKey a.SPK.publicKey := by
+  intro a
+  let h₁ := a.SPK
+  let k1 := a.SPK.publicKey
+  let k2 := a.SPK.privateKey
+  let h₂ := h₁.valid
+  exact h₂
+
+theorem match_bs_append {a1 a2 b1 b2 : ByteSequence} :
+  ∀ (bs1 bs2 : ByteSequence),
+    bs1 = ByteSequence.append a1 a2 →
+    bs2 = ByteSequence.append b1 b2 →
+    match_bs a1 b1 → match_bs a2 b2 → match_bs bs1 bs2 := by
+  intro bs1 bs2 h₁ h₂ h₃ h₄
+  rw [h₁, h₂]
+  simp [match_bs]
+  apply And.intro
+  repeat assumption
+
+theorem match_bs_dh {a1 a2 b1 b2 : Key} :
+  ∀ (bs1 bs2 : ByteSequence),
+    bs1 = ByteSequence.dh a1 a2 →
+    bs2 = ByteSequence.dh b1 b2 →
+    match_key a1 b1 → match_key a2 b2 → match_bs bs1 bs2 := by
+  intro bs1 bs2 h₁ h₂ h₃ h₄
+  rw [h₁, h₂]
+  simp [match_bs]
+  apply And.intro
+  repeat assumption
+
+
+theorem commonSharedSecret {a b : Agent} {txt : String}
+  (msg : Message) (h : b.OPKs = []) :
+  sendInitMessage a (toPublicBundle b) txt = Except.ok msg →
+  receiveInitMessage b msg = Except.ok txt := by
+  intro h₁
+  simp [sendInitMessage, receiveInitMessage,
+    toPublicBundle, toPrivateBundle, deriveSharedSecret,
+    decrypt, encrypt, generateKeyPair,
+    ByteSequence.append, makeMessage, verify,
+    match_bs] at *
+  have h₂ := all_agentIK₂ b
+  have h₃ := all_agentIK₂ a
+  have h₄ := all_agentSPK₂ b
+  have h₅ := all_agentSPK₂ a
+  simp [h₂, h₃, h₄, h₅, h] at h₁
+  simp [h₂, h]
+  rw [← h₁]
+  simp [match_bs_append, match_bs_dh]
+  sorry
+
 
 
 end X3DH
